tla-tree/ImmutableDiskTreeRefinement.dfy
@@ -30,7 +30,7 @@ function DiskView(k:Constants, s:Variables) : (diskView:View)
     ImmutableDiskTreeImpl.ViewOfDisk(s.disk.sectors)
 }
 
-predicate {:opaque} /*XXX*/ SysInv(k:Constants, s:Variables)
+predicate SysInv(k:Constants, s:Variables)
 {
     && WFDiskState(k, s)
     && TreeInv(k.impl, s.impl, DiskView(k, s))  // TODO remove this dependency until GC time
@@ -127,7 +127,7 @@ lemma TreeInvInduction(k:Constants, s:Variables, s':Variables, step:Step)
     assume false;    // TODO I think we're going to end up deleting TreeInv anyway.
 }
 
-function {:opaque} /*XXX*/ LookupForDatum(lv:LookupView, datum:Datum) : (lookup:ImmutableDiskTreeImpl.Lookup)
+function LookupForDatum(lv:LookupView, datum:Datum) : (lookup:ImmutableDiskTreeImpl.Lookup)
     requires datum in AllValueLookups(lv)
     ensures ValidValueLookup(lv, lookup)
     ensures ImmutableDiskTreeImpl.TerminalSlot(lookup).datum == datum
@@ -135,6 +135,15 @@ function {:opaque} /*XXX*/ LookupForDatum(lv:LookupView, datum:Datum) : (lookup:
     reveal_AllValueLookups();
     var lookup :| ValidValueLookup(lv, lookup) && ImmutableDiskTreeImpl.TerminalSlot(lookup).datum == datum;
     lookup
+}
+
+lemma LookupsMatch(lookup1:ImmutableDiskTreeImpl.Lookup, lookup2:ImmutableDiskTreeImpl.Lookup, len:int)
+    requires |lookup1.layers| == len;
+    requires |lookup2.layers| == len;
+    requires LookupsAgreeToLen(lookup1, lookup2, len);
+    ensures lookup1.layers == lookup2.layers;
+{
+    reveal_LookupsAgreeToLen();
 }
 
 lemma OneDatumPerKeyInvInduction(k:Constants, s:Variables, s':Variables, step:Step)
@@ -153,53 +162,58 @@ lemma OneDatumPerKeyInvInduction(k:Constants, s:Variables, s':Variables, step:St
         var lookup2 := LookupForDatum(lv, datum2);
         var commonPrefixLength := CommonPrefixOfLookups(lookup1, lookup2);
         if (commonPrefixLength == |lookup1.layers| == |lookup2.layers|) {
-            assert lookup1.layers == lookup2.layers;    // OBSERVE
-            assert lookup1 == lookup2;
-            calc {
-                datum1;
-                ImmutableDiskTreeImpl.TerminalSlot(lookup1).datum;
-                ImmutableDiskTreeImpl.TerminalSlot(lookup2).datum;
-                datum2;
-            }
+//            assert |lookup1.layers| == commonPrefixLength;
+            assert |lookup2.layers| == commonPrefixLength;  // The presence of this line CREATES a timeout. Wut?
+            //LookupsMatch(lookup1, lookup2, commonPrefixLength);
+//            assert lookup1.layers == lookup2.layers;    // OBSERVE
+//            assert lookup1 == lookup2;
+//            calc {
+//                datum1;
+//                ImmutableDiskTreeImpl.TerminalSlot(lookup1).datum;
+//                ImmutableDiskTreeImpl.TerminalSlot(lookup2).datum;
+//                datum2;
+//            }
+            assert datum1 == datum2;
         } else {
-            //assert LookupHonorsRanges(lookup1);
-            //assert LookupHonorsRanges(lookup2);
-            assert datum1 == ImmutableDiskTreeImpl.TerminalSlot(lookup1).datum;
-            assert datum2 == ImmutableDiskTreeImpl.TerminalSlot(lookup2).datum;
-//            if (commonPrefixLength == |lookup1.layers|) {
-//                //var termLayer1 := lookup1.layers[commonPrefixLength - 1];
-//                //assert termLayer1.node.slots[termLayer1.slot].Pointer?;
+//            //assert LookupHonorsRanges(lookup1);
+//            //assert LookupHonorsRanges(lookup2);
+//            assert datum1 == ImmutableDiskTreeImpl.TerminalSlot(lookup1).datum;
+//            assert datum2 == ImmutableDiskTreeImpl.TerminalSlot(lookup2).datum;
+////            if (commonPrefixLength == |lookup1.layers|) {
+////                //var termLayer1 := lookup1.layers[commonPrefixLength - 1];
+////                //assert termLayer1.node.slots[termLayer1.slot].Pointer?;
+////                assert false;
+////            }
+////            assert commonPrefixLength < |lookup1.layers|;
+//            if (commonPrefixLength == |lookup2.layers|) {
+//                var termLayer1 := lookup1.layers[commonPrefixLength - 1];
+//                //assert 0<=commonPrefixLength<|lookup1.layers|;
+//                assert ImmutableDiskTreeImpl.LookupHonorsPointerLinksAtLayer(lookup1, commonPrefixLength);  // OBSERVE
+//                assert commonPrefixLength - 1 != 0; // this line causes timeouts by itself!
+//                assert termLayer1.node.slots[termLayer1.slot].Pointer?;
+//
+//                var termLayer2 := lookup2.layers[commonPrefixLength - 1];
+//                assert termLayer2.node.slots[termLayer2.slot].Value?;
+//                /*
+//                assert ValidValueLookup(lv, lookup2);
+//                assert ImmutableDiskTreeImpl.ValidLookupInView(lv.k, lv.table, lv.view, lookup2);
+//                assert ImmutableDiskTreeImpl.LookupHonorsPointerLinks(lookup2);
+//                assert 0<=commonPrefixLength<|lookup2.layers|;
+//                assert ImmutableDiskTreeImpl.LookupHonorsPointerLinksAtLayer(lookup2, commonPrefixLength);
+//                assert termLayer2.node.slots[termLayer2.slot].Pointer?;
+//                */
 //                assert false;
 //            }
-//            assert commonPrefixLength < |lookup1.layers|;
-            if (commonPrefixLength == |lookup2.layers|) {
-                var termLayer1 := lookup1.layers[commonPrefixLength - 1];
-                //assert 0<=commonPrefixLength<|lookup1.layers|;
-                assert ImmutableDiskTreeImpl.LookupHonorsPointerLinksAtLayer(lookup1, commonPrefixLength);  // OBSERVE
-                assert commonPrefixLength - 1 != 0; // this line causes timeouts by itself!
-                assert termLayer1.node.slots[termLayer1.slot].Pointer?;
-
-                var termLayer2 := lookup2.layers[commonPrefixLength - 1];
-                assert termLayer2.node.slots[termLayer2.slot].Value?;
-                /*
-                assert ValidValueLookup(lv, lookup2);
-                assert ImmutableDiskTreeImpl.ValidLookupInView(lv.k, lv.table, lv.view, lookup2);
-                assert ImmutableDiskTreeImpl.LookupHonorsPointerLinks(lookup2);
-                assert 0<=commonPrefixLength<|lookup2.layers|;
-                assert ImmutableDiskTreeImpl.LookupHonorsPointerLinksAtLayer(lookup2, commonPrefixLength);
-                assert termLayer2.node.slots[termLayer2.slot].Pointer?;
-                */
-                assert false;
-            }
-            assert commonPrefixLength < |lookup2.layers|;
-            assert false;
-            assert commonPrefixLength < |lookup2.layers|;   // Else commonPrefixLength slot isn't a Value.
-
-            assert lookup1.layers[commonPrefixLength].node == lookup2.layers[commonPrefixLength].node;
-            assert lookup1.layers[commonPrefixLength].slot != lookup2.layers[commonPrefixLength].slot;
-            assert lookup1.layers[commonPrefixLength].slotRange != lookup2.layers[commonPrefixLength].slotRange;
-            // They're going to have different ranges.
-            //assume false;
+//            assert commonPrefixLength < |lookup2.layers|;
+//            assert false;
+//            assert commonPrefixLength < |lookup2.layers|;   // Else commonPrefixLength slot isn't a Value.
+//
+//            assert lookup1.layers[commonPrefixLength].node == lookup2.layers[commonPrefixLength].node;
+//            assert lookup1.layers[commonPrefixLength].slot != lookup2.layers[commonPrefixLength].slot;
+//            assert lookup1.layers[commonPrefixLength].slotRange != lookup2.layers[commonPrefixLength].slotRange;
+//            // They're going to have different ranges.
+//            //assume false;
+            assert datum1 == datum2;
         }
     }
 }
